src/HWIface.fsti
@@ -43,9 +43,11 @@ val alg : dice_alg
 
 let digest_length = hash_len alg
 
-val uds_length : l: uint_32 {v l <= max_input_length alg}
+val uds_length : l: uint_32 {v l <= max_input_length alg /\ v l > 0}
 
 let cdi_length = digest_length
+
+let riot_size_t = i: uint_32{v i <= max_input_length alg /\ v i > 0}
 
 /// The model maintains some abstract local state
 ///
@@ -82,8 +84,13 @@ val uds_is_disabled : Type0
 /// The state provides getters for UDS and CDI (see below)
 ///   so the native implementation can implement it simply as a record of two pointers (uds and cdi)
 
-val state : Type0
+noeq
+type riot_t = {
+  size  : riot_size_t;
+  binary: b: B.buffer uint8{B.length b == v size /\ B.freeable b}
+}
 
+val state : Type0
 
 /// Clients can get the uds and the cdi buffer from the state
 ///   And also value of the UDS for the purposed of the spec
@@ -94,6 +101,9 @@ val get_uds (st:state)
 val get_cdi (st:state)
 : Tot (b:B.buffer uint8{B.length b == v cdi_length /\ B.freeable b})
 
+val get_riot (st:state)
+: Tot (r:riot_t)
+
 val get_uds_value (st:state)
 : GTot (s:Seq.seq uint8{Seq.length s == v uds_length})
 
@@ -101,20 +111,24 @@ val get_uds_value (st:state)
 
 unfold
 let get_buf_t_l st = [ B.buf (get_uds st)
-                     ; B.buf (get_cdi st) ]
+                     ; B.buf (get_cdi st)
+                     ; B.buf (get_riot st).binary ]
 
 unfold
 let get_loc_l st = [ B.loc_buffer (get_uds st)
-                   ; B.loc_buffer (get_cdi st) ]
+                   ; B.loc_buffer (get_cdi st)
+                   ; B.loc_buffer (get_riot st).binary ]
 
 unfold
 let get_buf_l st = [ get_uds st
-                   ; get_cdi st ]
+                   ; get_cdi st
+                   ; (get_riot st).binary ]
 
 unfold
 let contains (h:HS.mem) (st:state) =
   B.live h (get_uds st) /\
-  B.live h (get_cdi st)
+  B.live h (get_cdi st) /\
+  B.live h (get_riot st).binary
 
 
 /// The initialization routine
@@ -132,20 +146,21 @@ let contains (h:HS.mem) (st:state) =
 /// TODO: this currently does not say anything about the allocations it does
 ///       e.g. this function is currently allowed to allocate two uds buffers and copy UDS into them
 
-val initialize (_:unit)
+val initialize
+  (riot_size: riot_size_t)
 : ST state
   (requires fun h -> uds_is_uninitialized h)
   (ensures fun h0 st h1 ->
     uds_is_initialized /\  //uds has been initialized
     (let (| _, _, local_st |) = local_state in
-     let uds = get_uds st in
-     let cdi = get_cdi st in
+     let uds  = get_uds st in
+     let cdi  = get_cdi st in
+     let riot = get_riot st in
      HS.contains h1 local_st /\
      B.(modifies (loc_mreference local_st) h0 h1) /\
      h1 `contains` st /\
-     B.disjoint uds cdi /\
-     B.(loc_disjoint (loc_buffer uds) (loc_mreference local_st)) /\
-     B.(loc_disjoint (loc_buffer cdi) (loc_mreference local_st)) /\
+     B.all_disjoint (get_loc_l st `FStar.List.Tot.append` [B.loc_mreference local_st]) /\
+     riot.size == riot_size /\
      B.as_seq h1 uds == get_uds_value st))
 
 
